Remove var cases from nsequiv
nsequiv used to have constructors for `nsequiv (var X) S` and
`nsequiv S (var X)`, which I thought were necessary for proving nsequiv
and `fun S S' => ~ sequiv S S'` equivalent. Turns out this is not the
case, and removing these constructors should make proofs by induction
over a derivation for `nsequiv S S'` easier.

NonEquivalence.v
@@ -43,12 +43,6 @@ Inductive nsequiv : Sty -> Sty -> Prop :=
     forall X S S',
     nsequiv S (subst X (mu X S') S') ->
     nsequiv S (mu X S')
-| nsequiv_var_l :
-    forall X S',
-    nsequiv (var X) S'
-| nsequiv_var_r :
-    forall X S,
-    nsequiv S (var X)
 | nsequiv_shape :
     forall S S',
     shape S  <> muS ->
